separate out Sector from Statemodel

Impl/StateModel.i.dfy
@@ -84,12 +84,7 @@ module StateModel {
 
   datatype Variables = Variables(
     bc: BCVariables,
-    jc: CommitterModel.CM)
-
-  datatype Sector =
-    | SectorNode(node: Node)
-    | SectorIndirectionTable(indirectionTable: IndirectionTable)
-    | SectorSuperblock(superblock: SectorType.Superblock)
+    jc: Committer)
 
   predicate IsLocAllocIndirectionTable(indirectionTable: IndirectionTable, i: int)
   {
@@ -161,18 +156,6 @@ module StateModel {
   {
     && (vars.Ready? ==> WFVarsReady(vars))
   }
-  predicate WFSector(sector: Sector)
-  {
-    match sector {
-      case SectorNode(node) => WFNode(node)
-      case SectorIndirectionTable(indirectionTable) => (
-        && IndirectionTableModel.Inv(indirectionTable)
-        && BC.WFCompleteIndirectionTable(IIndirectionTable(indirectionTable))
-      )
-      case SectorSuperblock(superblock) =>
-        JC.WFSuperblock(superblock)
-    }
-  }
 
   function INode(node: Node) : (result: BT.G.Node)
   {
@@ -203,15 +186,6 @@ module StateModel {
       case LoadingIndirectionTable(loc, read) =>
         BC.LoadingIndirectionTable(loc, read)
       case Unready => BC.Unready
-    }
-  }
-  function ISector(sector: Sector) : SectorType.Sector
-  requires WFSector(sector)
-  {
-    match sector {
-      case SectorNode(node) => SectorType.SectorNode(INode(node))
-      case SectorIndirectionTable(indirectionTable) => SectorType.SectorIndirectionTable(IIndirectionTable(indirectionTable))
-      case SectorSuperblock(superblock) => SectorType.SectorSuperblock(superblock)
     }
   }
 
