Impl/StateSectorModel.i.dfy
@@ -1,0 +1,43 @@
+include "../PivotBetree/PivotBetreeSpec.i.dfy"
+include "IndirectionTableModel.i.dfy"
+include "../BlockCacheSystem/SectorType.i.dfy"
+include "../BlockCacheSystem/JournalCache.i.dfy"
+
+module StateSectorModel {
+  import BT = PivotBetreeSpec`Internal
+  import IndirectionTableModel
+  import SectorType
+  import BC = BlockCache
+  import JC = JournalCache
+
+  type Node = BT.G.Node  
+
+  datatype Sector =
+    | SectorNode(node: Node)
+    | SectorIndirectionTable(indirectionTable: IndirectionTableModel.IndirectionTable)
+    | SectorSuperblock(superblock: SectorType.Superblock)
+
+  predicate WFSector(sector: Sector)
+  {
+    match sector {
+      case SectorNode(node) => BT.WFNode(node)
+      case SectorIndirectionTable(indirectionTable) => (
+        && IndirectionTableModel.Inv(indirectionTable)
+        && BC.WFCompleteIndirectionTable(IndirectionTableModel.I(indirectionTable))
+      )
+      case SectorSuperblock(superblock) =>
+        JC.WFSuperblock(superblock)
+    }
+  }
+
+  function ISector(sector: Sector) : SectorType.Sector
+  requires WFSector(sector)
+  {
+    match sector {
+      case SectorNode(node) => SectorType.SectorNode(BT.G.Node(node.pivotTable, node.children, node.buckets))
+      case SectorIndirectionTable(indirectionTable) =>
+        SectorType.SectorIndirectionTable(IndirectionTableModel.I(indirectionTable))
+      case SectorSuperblock(superblock) => SectorType.SectorSuperblock(superblock)
+    }
+  }
+}
